Update progress file
Now instead of picking a particular thing to do, progress is taking its
proper place as the computational reflection of the step relation.

mltt-in-coq/Progress.v
@@ -1,21 +1,77 @@
+Require Import Coq.Program.Program List.
+Import ListNotations.
+Require Import Monad Tactics.
 Require Import Unscoped Evaluation.
-Theorem progress : forall e, {e' | e ==> e'} + {forall e', ~e ==> e'}.
-  induction e; repeat (destr_sumors; try (destr_exists; left; eauto)); 
-  try (right; inversion 1; subst; try_hyps; contradiction);
-  match goal with
-    | [|-context[?e1 @ ?e2]] => destruct e1
-    | [|-context[srec _ _ ?e3]] => destruct e3
-    | [|-context[wrec _ _ ?e3]] => destruct e3
-    | [|-context[urec _ _ ?e3]] => destruct e3
-    | [|-context[brec _ _ _ ?e4]] => destruct e4
-  end;        
-  match goal with
-    | [|-context[lam _ ?b @ ?e2]] => left; exists (b |> e2 // 0); auto
-    | [|-context[srec _ ?e2 (?a # ?b)]] => left; exists (e2 @ a @ b); auto
-    | [|-context[wrec _ ?e2 (sup _ ?a ?f)]] => left; eauto
-    | [|-context[urec _ ?u unit]] => left; exists u; auto
-    | [|-context[brec _ ?t ?f true]] => left; exists t; auto
-    | [|-context[brec _ _ ?f false]] => left; exists f; auto
-    | _ => right; inversion 1; subst; try_hyps; contradiction
-  end.
+
+Fixpoint progress (e: exp) : list exp :=
+  join
+    match e with
+      | pi A B => [pi <$> progress A <*> pure B; pi A <$> progress B]
+      | lam A b => [lam <$> progress A <*> pure b; lam A <$> progress b]
+      | app f x => [app <$> progress f <*> pure x; app f <$> progress x
+                   ; match f with lam A b => pure (b |> x // 0) | _ => [] end]
+
+      | sigma A B => [sigma <$> progress A <*> pure B; sigma A <$> progress B]
+      | smk B a b => [smk <$> progress B <*> pure a <*> pure b; smk B <$> progress a <*> pure b; smk B a <$> progress b]
+      | srec C p s => [srec <$> progress C <*> pure p <*> pure s; srec C <$> progress p <*> pure s; srec C p <$> progress s; 
+                      match s with (a # b) => pure (p @ a @ b) | _ => [] end]
+
+      | wt A B => [wt <$> progress A <*> pure B; wt A <$> progress B]
+      | sup B a f => [sup <$> progress B <*> pure a <*> pure f; sup B <$> progress a <*> pure f; sup B a <$> progress f]
+      | wrec C s w => [wrec <$> progress C <*> pure s <*> pure w; wrec C <$> progress s <*> pure w; wrec C s <$> progress w;
+                      match w with
+                        | (sup B a f) => pure (s @ a @ lam (B @ a) (wrec (wk_deep 1 0 C) (wk_deep 1 0 s) (wk_deep 1 0 f @ &0)))
+                        | _ => []
+                      end]
+
+      | brec C t f b => [brec <$> progress C <*> pure t <*> pure f <*> pure b; brec C <$> progress t <*> pure f <*> pure b;
+                        brec C t <$> progress f <*> pure b; brec C t f <$> progress b;
+                        match b with true => pure t | false => pure f | _ => [] end]
+      | urec C u t => [urec <$> progress C <*> pure u <*> pure t; urec C <$> progress u <*> pure t; urec C u <$> progress t;
+                      match t with unit => pure u | _ => [] end]
+
+      | exf C f => [exf <$> progress C <*> pure f; exf C <$> progress f]
+      | _ => []
+    end.
+
+Lemma join_fmap_unit M `(Monad M) A B x (xs: M (A -> B)) : join ((fun f => pure (f x)) <$> xs) = ((fun f => f x) <$> xs).
+  replace (fun f => pure (f x)) with (@pure M H B ∘ (fun f => f x)) by auto; rewrite hom_comp; auto. Qed.
+
+Definition concat_unit : forall A B x xs, concat (map (fun (f: A -> B) => [f x]) xs) = map (fun f => f x) xs := join_fmap_unit list list_monad.
+
+Definition in_concat A x xss : @In A x (concat xss) <-> exists xs, In xs xss /\ In x xs.
+  induction xss; split; simpl; try (inversion 1; subst; auto); intros; try (destr_logic; auto; fail).
+  - apply in_app_or in H; destr_logic; eauto. try_hyps; destr_logic; eauto.
+  - destr_logic; repeat subst; apply in_or_app; try (left;eauto;fail); right.
+    + apply IHxss; eauto.
 Qed.
+
+Hint Resolve in_eq.
+
+Theorem progress_exhaustive : forall e1 e2, e1 ==> e2 -> In e2 (progress e1).
+  induction 1; intros; simpl; try (simpl in *; auto; fail); 
+  (* some simplifying rewrites *)
+  repeat (rewrite concat_unit || rewrite map_map || rewrite map_app); auto;
+  (* now we'll elim all the simple recursive cases *)
+  try (repeat 
+         ((apply in_or_app; left; match goal with [|-In _ (map ?e _)] => apply in_map with (f := e) end; auto; fail)
+         || (apply in_or_app; right)); fail);
+  (* elim rules will then live in the last part of the list *)
+  try (repeat (apply in_or_app; right); auto; fail).
+Qed. 
+
+Theorem progress_faithful : forall e1 e2, In e2 (progress e1) -> e1 ==> e2.
+  induction e1; intros.
+Admitted.
+
+Reserved Notation "e1 =[ n ]=> e2" (at level 50).
+Inductive n_steps e1 : nat -> exp -> Prop :=
+| n_stop : e1 =[0]=> e1
+| n_back : forall e2 e3 n, e1 ==> e2 -> e2 =[n]=> e3 -> e1 =[S n]=> e3
+where "e1 =[ n ]=> e2" := (n_steps e1 n e2).
+Hint Constructors n_steps.
+
+Lemma n_step e1 e2 e3 n : e1 =[n]=> e2 -> e2 ==> e3 -> e1 =[S n]=> e3.
+  induction 1; eauto. Qed.
+
+Hint Resolve n_step.
